WIP Beginnings of first refinement

compiler/backend/gc/generational_gcScript.sml
@@ -7,7 +7,7 @@ val gc_state_component_equality = DB.fetch "gc_shared" "gc_state_component_equal
 val _ = Datatype `
   gen_gc_conf =
     <| limit : num              (* size of heap *)
-     ; isRef : ('a, 'b) heap_element -> bool
+     ; isRef : 'a -> bool
      ; gen_start : num          (* start of generation *)
      ; gen_end : num            (* end of generation *)
      ; refs_start : num         (* start of references, gen_end < refs_start *)
@@ -16,22 +16,18 @@ val _ = Datatype `
 val gc_move_def = Define `
   (gc_move conf state (Data d) = (Data d, state)) /\
   (gc_move conf state (Pointer ptr d) =
-     if ptr < conf.gen_start \/ conf.gen_end <= ptr then
-       let (heap, ok) =  gc_forward_ptr ptr state.heap ptr d state.ok in
-       (Pointer ptr d
-       ,state with <| heap := heap; ok := ok |>) else
+     if ptr < conf.gen_start \/ conf.refs_start <= ptr then
+       (Pointer ptr d,state) else
      case heap_lookup ptr state.heap of
      | SOME (DataElement xs l dd) =>
        let ok = state.ok /\ l+1 <= state.n in
        let n = state.n - (l + 1) in
-        if conf.isRef (DataElement xs l dd) then
-          (* put refs in r4 *)
+        if conf.isRef dd then
           let r4 = (DataElement xs l dd) :: state.r4 in
-          let (heap, c) = gc_forward_ptr ptr state.heap (state.a + n) d ok in
+          let (heap,ok) = gc_forward_ptr ptr state.heap (state.a + n) d ok in
             (Pointer (state.a + n) d
             ,state with <| r4 := r4; n := n; heap := heap; ok := ok |>)
         else
-          (* put data in h2 *)
           let h2 = state.h2 ++ [DataElement xs l dd] in
           let (heap,ok) = gc_forward_ptr ptr state.heap state.a d ok in
           let a = state.a + l + 1 in
@@ -49,11 +45,9 @@ val gc_move_consts = prove(
     (state.r1 = state'.r1)``,
   Cases
   \\ fs [gc_move_def]
-  \\ ntac 4 strip_tac
-  \\ Cases_on `n < conf.gen_start ∨ conf.gen_end ≤ n`
-  THEN1
-    (pairarg_tac \\ fs []
-    \\ fs [gc_state_component_equality])
+  \\ ntac 3 strip_tac
+  \\ IF_CASES_TAC >- fs [gc_state_component_equality]
+  \\ strip_tac
   \\ fs []
   \\ Cases_on `heap_lookup n state.heap`
   \\ fs [gc_state_component_equality]
@@ -61,7 +55,7 @@ val gc_move_consts = prove(
   \\ fs [LET_THM,gc_state_component_equality]
   \\ pairarg_tac
   \\ fs []
-  \\ Cases_on `conf.isRef (DataElement l n' b)`
+  \\ Cases_on `conf.isRef b`
   \\ pairarg_tac
   \\ fs [gc_state_component_equality]);
 
@@ -152,7 +146,7 @@ val partial_gc_def = Define `
                 ; a := conf.gen_start; n := n |> in
         (* process roots: *)
       let (roots,state) = gc_move_list conf state roots in
-        (* process references: *)
+        (* process roots from references: *)
       let state = gc_move_refs conf state in
         (* process rest: *)
       let state = gc_move_loop conf state conf.limit in
@@ -162,7 +156,8 @@ val partial_gc_def = Define `
       (*          (heap_length state.heap = conf.limit) /\ *)
       (*          (state.a + state.n + state.r = conf.limit) /\ *)
       (*          state.a + state.r <= conf.limit in *)
-          (roots,state)`;
+      let state = state with <|h1 := old ++ state.h1|> in
+      (roots,state)`; (* TODO: old? *)
 
 val full_gc_def = Define `
   full_gc conf (roots,heap) =
@@ -179,9 +174,9 @@ val heap_gen_ok_def = Define `
       (!ptr xs l d u. MEM (DataElement xs l d) old /\ MEM (Pointer ptr u) xs ==>
         (ptr < conf.gen_start \/ conf.gen_end <= ptr)) /\
       (* old contains no references *)
-      (!el. MEM el old ==> ~ (conf.isRef el)) /\
+      (!xs l d. MEM (DataElement xs l d) old ==> ~ (conf.isRef d)) /\
       (* refs only contains references *)
-      (!el. MEM el refs ==> conf.isRef el)`;
+      (!xs l d. MEM (DataElement xs l d) refs ==> conf.isRef d)`;
 
 val _ = Datatype `
   data_sort = Protected 'a      (* actually a pointer to an older generation *)
@@ -202,16 +197,16 @@ val to_gen_heap_address_def = Define `
   (to_gen_heap_address gen_start (Data (Real b)) = Data b) /\
   (to_gen_heap_address gen_start (Pointer ptr (Real a)) = Pointer (ptr + gen_start) a)`;
 
-val to_basic_isRef_def = Define `
-  (to_basic_isRef isRef (DataElement ptrs n d) =
-    isRef (DataElement (MAP (to_gen_heap_address 0) ptrs) n d)) /\
-  (to_basic_isRef isRef _ = F)`;
+(* val to_basic_isRef_def = Define ` *)
+(*   (to_basic_isRef isRef d = *)
+(*     isRef (DataElement (MAP (to_gen_heap_address 0) ptrs) n d)) /\ *)
+(*   (to_basic_isRef isRef _ = F)`; *)
 
 val to_basic_conf_def = Define `
-  to_basic_conf (conf:('a,'b) gen_gc_conf) =
+  to_basic_conf (conf:'a gen_gc_conf) =
     <| limit := conf.limit
-     ; isRef := to_basic_isRef conf.isRef |>
-     : (('a heap_address, 'a) data_sort, 'b) basic_gc_conf`;
+     ; isRef := conf.isRef |>
+     : 'a basic_gc_conf`;
 
 val to_basic_heap_element_def = Define `
   (to_basic_heap_element conf (Unused n) = Unused n) /\
@@ -220,19 +215,30 @@ val to_basic_heap_element_def = Define `
   (to_basic_heap_element conf (DataElement ptrs l d) =
     DataElement (MAP (to_basic_heap_address conf) ptrs) l d)`;
 
+val restrict_heap_def = Define `
+  restrict_heap start end (heap:('a,'b) heap_element list) =
+     case heap_segment (start,end) heap of
+     | NONE => ARB
+     | SOME (h1,h2,h3) => h2`;
+
+val to_basic_heap_list_def = Define `
+  to_basic_heap_list conf heap =
+    MAP (to_basic_heap_element conf) heap`;
+
 val to_basic_heap_def = Define `
   to_basic_heap conf heap =
-    MAP (to_basic_heap_element conf) (heap_drop conf.gen_start heap)`;
+    to_basic_heap_list conf
+        (restrict_heap conf.gen_start conf.refs_start heap)`;
 
 val to_basic_state_def = Define `
   to_basic_state conf state =
     empty_state with
-    <| h1 := MAP (to_basic_heap_element conf) state.h1
-     ; h2 := MAP (to_basic_heap_element conf) state.h2
-     ; r4 := MAP (to_basic_heap_element conf) state.r4
-     ; r3 := MAP (to_basic_heap_element conf) state.r3
-     ; r2 := MAP (to_basic_heap_element conf) state.r2
-     ; r1 := MAP (to_basic_heap_element conf) state.r1
+    <| h1 := to_basic_heap_list conf state.h1
+     ; h2 := to_basic_heap_list conf state.h2
+     ; r4 := to_basic_heap_list conf state.r4
+     ; r3 := to_basic_heap_list conf state.r3
+     ; r2 := to_basic_heap_list conf state.r2
+     ; r1 := to_basic_heap_list conf state.r1
      ; a := state.a - conf.gen_start
      ; n := state.n
      ; ok := state.ok
@@ -299,24 +305,128 @@ val RootsRefs_related = prove(
   \\ simp [r2r_filter_def]
   \\ metis_tac [RootsRefs_cases]);
 
-val simulation = prove(
-  ``!broots' bstate'.
-    let bheap = to_basic_heap conf heap in
-    let broots = to_basic_roots conf.gen_start roots ++
-                 refs_to_roots (heap_drop conf.refs_start bheap) in
-    (basic_gc (to_basic_conf conf) (broots,bheap) = (broots',bstate')) ==>
-    ?roots' state'.
-      (partial_gc conf (roots, heap) = (roots',state')) /\
-      (TAKE (LENGTH roots) broots' = to_basic_roots conf.gen_start roots') /\
-      (bstate' = to_basic_state conf state')(*  /\ *)
-      (* (RootsRefs (heap_drop conf.refs_start state. (DROP (LENGTH roots) roots')) *)``,
+(*
+
+     GenGC     GC
+inp    o ----> o
+       |       |
+       |       |
+       v       v
+out    o ----> o
+
+last step: need a relation <---
+ *)
+
+val gen_inv_def = Define `
+  gen_inv (conf:'b gen_gc_conf) heap =
+    !h1 h2 h3 (* h10 h20 h30 *).
+    (heap_segment (conf.gen_start,conf.refs_start) heap = SOME (h1,h2,h3))(*  /\ *)
+    (* (heap_segment (conf.gen_start,conf.refs_start) state.heap0 = SOME (h10,h20,h30)) *)`;
+
+(* val gc_forward_ptr_gen_inv = prove( *)
+(*   ``!state state' conf n ptr a ok. *)
+(*     gen_inv conf state /\ *)
+(*     (gc_forward_ptr n state.heap ptr a state.ok = (heap',ok')) ==> *)
+(*     gen_inv conf (state with <|heap:=heap';ok:=ok'|>)``, *)
+(*   cheat); *)
+(*   (* Induct_on `state.heap` *) *)
+(*   (* \\ rw [] *) *)
+(*   (* \\ qpat_x_assum `_ = state.heap` (assume_tac o GSYM) \\ fs [] *) *)
+(*   (* \\ fs [gc_forward_ptr_def,gen_inv_def] *) *)
+(*   (* \\ qpat_x_assum `_ = (heap',ok')` mp_tac *) *)
+(*   (* \\ IF_CASES_TAC \\ fs [] *) *)
+(*   (* >- (strip_tac *) *)
+(*   (*    \\ qpat_x_assum `_ = heap'` (assume_tac o GSYM) \\ fs [] *) *)
+(*   (*    \\ rpt strip_tac *) *)
+(*   (*    \\ fs [heap_segment_def,heap_split_def,el_length_def] *) *)
+(*   (*    \\ fs []) *) *)
+(*   (* cheat); *) *)
+
+val gc_move_heap_lookup_lemma = prove(
+  ``!heap n conf.
+    ¬(n < conf.gen_start) /\
+    ¬(conf.refs_start ≤ n) /\
+    (heap_lookup (n − conf.gen_start) (to_basic_state conf state).heap
+     = OPTION_MAP ()) ==>
+    (heap_lookup n state.heap = NONE)
+
+val gc_move_simulation = prove(
+  ``!ptr ptr' state state'.
+      gen_inv conf state.heap /\
+      (gc_move conf state ptr = (ptr', state')) ==>
+      (gen_inv conf state'.heap) /\
+      (basic_gc$gc_move
+         (to_basic_conf conf)
+         (to_basic_state conf state)
+         (to_basic_heap_address conf ptr)
+       = (to_basic_heap_address conf ptr', to_basic_state conf state'))``,
+
+  reverse Cases
+  \\ ntac 4 strip_tac
+  \\ fs [to_basic_heap_address_def]
+  >- (fs [gc_move_def,basic_gcTheory.gc_move_def]
+     \\ qpat_x_assum `Data a = _` (assume_tac o GSYM)
+     \\ fs [to_basic_heap_address_def])
+  \\ IF_CASES_TAC
+  >- (fs [gc_move_def,basic_gcTheory.gc_move_def,gen_inv_def]
+     \\ qpat_x_assum `_ = ptr'` (assume_tac o GSYM) \\ fs []
+     \\ fs [to_basic_heap_address_def])
+  \\ IF_CASES_TAC
+  >- (fs [gc_move_def,basic_gcTheory.gc_move_def,gen_inv_def]
+     \\ qpat_x_assum `_ = ptr'` (assume_tac o GSYM) \\ fs []
+     \\ fs [to_basic_heap_address_def])
+  \\ fs [gc_move_def,basic_gcTheory.gc_move_def,gen_inv_def]
+  \\ strip_tac >- cheat
+  \\ BasicProvers.TOP_CASE_TAC \\ fs []
+  >- (`heap_lookup n state.heap = NONE` by all_tac
+     >- (pop_assum mp_tac
+        \\ Induct_on
+        \\ fs [heap_lookup_def]
+        \\
+     )
+  )
+  \\ cheat
+  );
+
+val gc_move_list_simulation = prove(
+  ``!conf state xs state' xs'.
+    (gc_move_list conf state xs = (xs', state')) ==>
+    (basic_gc$gc_move_list (to_basic_conf conf) (to_basic_state conf state)
+                           (MAP (to_basic_heap_address conf) xs)
+    = (MAP (to_basic_heap_address conf) xs', to_basic_state conf state'))``,
   cheat);
 
-(*
-- basic_gc_related
-1 simulering: from_gen_..., m cheat
-2 partial_gc_related, m antagande om inga pointers i fel riktigt (generationer)
- *)
+val RootsRel = Hol_reln `
+  (!a b. RootsRel [Pointer 12 a] [Pointer 13 b])`;
+
+val StateRel = Hol_reln `
+  (!conf. StateRel (to_basic_state conf empty_state) empty_state)`;
+
+val simulation_thm = store_thm("simulation_thm",
+  ``!roots heap conf.
+      (SOME refs = OPTION_MAP (refs_to_roots o SND) (heap_split conf.refs_start state.heap)) /\
+      (basic_gc (to_basic_conf conf)
+                (to_basic_roots conf.gen_start roots ++ refs, to_basic_heap conf heap)
+       = (bRoots',bState')) ==>
+      ?roots' state'.
+        (partial_gc conf (roots,heap) = (roots',state')) /\
+        (StateRel bState' state') /\
+        (RootsRel bRoots' roots')``,
+  cheat);
+
+
+(* val simulation = prove( *)
+(*   ``!broots' bstate'. *)
+(*     let bheap = to_basic_heap conf heap in *)
+(*     let broots = to_basic_roots conf.gen_start roots ++ *)
+(*                  refs_to_roots (heap_drop conf.refs_start bheap) in *)
+(*     (basic_gc (to_basic_conf conf) (broots,bheap) = (broots',bstate')) ==> *)
+(*     ?roots' state'. *)
+(*       (partial_gc conf (roots, heap) = (roots',state')) /\ *)
+(*       (TAKE (LENGTH roots) broots' = to_basic_roots conf.gen_start roots') /\ *)
+(*       (bstate' = to_basic_state conf state')(*  /\ *) *)
+(*       (* (RootsRefs (heap_drop conf.refs_start state. (DROP (LENGTH roots) roots')) *)``, *)
+(*   cheat); *)
 
 val fmap_fun_def = Define `
   fmap_fun (f:num |-> num) gen_start heap =
@@ -356,14 +466,63 @@ val fmap_fun_LESS_gen_start = prove(
     (fmap_fun f gen_start heap ' n = n)``,
   fs [fmap_fun_def,FUN_FMAP_DEF]);
 
+val partial_gc_simulation = prove(
+  ``(partial_gc conf (roots,heap) = (roots1,state1)) /\
+    roots_ok roots (heap:('a,'b) heap_element list) /\
+    heap_ok heap conf.limit /\
+    heap_gen_ok heap conf /\
+    (SOME refs = OPTION_MAP (refs_to_roots o SND) (heap_split conf.refs_start heap)) ==>
+    (basic_gc (to_basic_conf conf)
+              (to_basic_roots conf.gen_start roots ++ MAP (to_basic_heap_address conf) refs,
+               MAP (to_basic_heap_element conf) (restrict_heap conf.gen_start conf.refs_start heap))
+     = (to_basic_roots conf.gen_start roots1, (* TODO: add refs roots *)
+       to_basic_state conf state1))``,
+  rpt strip_tac
+  cheat);
+
+val f_old_ptrs_def = Define `
+  f_old_ptrs conf heap = {a | isSomeDataElement (heap_lookup a heap)
+                              /\ (a < conf.gen_start \/ conf.refs_start <= a)}`;
+
+val new_f_def = Define `
+  new_f f conf heap =
+    FUNION (FUN_FMAP I (f_old_ptrs conf heap))
+           (FUN_FMAP (\a. conf.gen_start + f ' (a - conf.gen_start))
+                     (IMAGE ((+) conf.gen_start) (FDOM f)))`;
+
 val partial_gc_related = store_thm("partial_gc_related",
-  ``roots_ok roots heap /\ heap_ok (heap:('a,'b) heap_element list) conf.limit /\
-    heap_gen_ok heap conf ==>
+  ``roots_ok roots heap /\
+    heap_ok (heap:('a,'b) heap_element list) conf.limit /\
+    heap_gen_ok heap conf /\
+    gen_inv conf heap ==>
     ?state f.
       (partial_gc conf (roots:'a heap_address list,heap) =
          (ADDR_MAP (FAPPLY f) roots,state)) /\
       (!ptr u. MEM (Pointer ptr u) roots ==> ptr IN FDOM f) /\
+      (heap_ok (state.h1 ++ heap_expand state.n ++ state.r1) conf.limit) /\
       gc_related f heap (state.h1 ++ heap_expand state.n ++ state.r1)``,
+
+  rpt strip_tac
+  \\ Cases_on `partial_gc conf (roots,heap)` \\ fs []
+  \\ rename1 `_ = (roots1,state1)`
+  \\ drule partial_gc_simulation
+  \\ fs []
+  \\ impl_tac
+  >- cheat
+  \\ strip_tac
+  \\ qabbrev_tac `basic_roots = to_basic_roots conf.gen_start roots ++ MAP (to_basic_heap_address conf) refs`
+  \\ qabbrev_tac `basic_heap = MAP (to_basic_heap_element conf) (restrict_heap conf.gen_start conf.refs_start heap)`
+  (* \\ qispecl_then  *)
+  \\ qspecl_then
+      [`basic_roots`,`basic_heap`,`to_basic_conf conf`] mp_tac
+      (basic_gc_related |> INST_TYPE [``:'a`` |-> ``:('a heap_address, 'a) data_sort``])
+  \\ impl_tac
+  >- cheat
+  \\ strip_tac \\ fs []
+  \\ qexists_tac `new_f f conf heap`
+  \\
+
+
   cheat);
   (* rpt strip_tac *)
   (* \\ mp_tac simulation *)
@@ -426,6 +585,7 @@ val full_gc_related = store_thm("full_gc_related",
     ?state f.
       (full_gc conf (roots:'a heap_address list,heap) =
          (ADDR_MAP (FAPPLY f) roots,state)) /\
+      (heap_ok (state.h1 ++ heap_expand state.n ++ state.r1) conf.limit) /\
       (!ptr u. MEM (Pointer ptr u) roots ==> ptr IN FDOM f) /\
       gc_related f heap (state.h1 ++ heap_expand state.n ++ state.r1)``,
   cheat);
